Precompute the message schedule

code/hash/Hacl.SHA2.fst
@@ -125,29 +125,98 @@ let init_512: init_t SHA2_512 =
 let block_w (a: sha2_alg) =
   b:B.buffer (word a) { B.length b = size_block_w }
 
+let ws_w a = b:B.buffer (word a) { B.length b = Spec.size_k_w a }
+
+val ws (a: sha2_alg) (b: block_w a) (ws: ws_w a):
+  ST.Stack unit
+    (requires (fun h ->
+      B.live h b /\ B.live h ws /\ B.disjoint b ws))
+    (ensures (fun h0 _ h1 ->
+      let b = B.as_seq h0 b in
+      M.(modifies (loc_buffer ws) h0 h1) /\
+      B.as_seq h1 ws == S.init (Spec.size_k_w a) (Spec.ws a b)))
+
+// A detour with three sequence lemmas required for the proof below to go through.
+
+let init_next (#a: Type) (s: S.seq a) (f: (i:nat { i < S.length s }) -> a) (i: nat):
+  Lemma
+    (requires (
+      i < S.length s /\
+      S.equal (S.slice s 0 i) (S.init i f) /\
+      S.index s i == f i))
+    (ensures (S.equal (S.slice s 0 (i + 1)) (S.init (i + 1) f)))
+=
+  admit ()
+
+let init_index (#a: Type) (j: nat) (f: (i:nat { i < j }) -> a) (i: nat):
+  Lemma
+    (requires (
+      i < j))
+    (ensures (S.index (S.init j f) i == f i))
+  [ SMTPat (S.index (S.init j f) i) ]
+=
+  ()
+
+let index_slice (#a: Type) (s: S.seq a) (j: nat) (i: nat):
+  Lemma
+    (requires (
+      i < j /\ j <= S.length s))
+    (ensures (S.index (S.slice s 0 j) i == S.index s i))
+  [ SMTPat (S.index (S.slice s 0 j) i) ]
+=
+  ()
+
 #set-options "--max_fuel 1"
 
-val ws (a: sha2_alg) (b: block_w a) (t: U32.t { U32.v t < Spec.size_k_w a }):
-  ST.Stack (word a)
-    (requires (fun h -> B.live h b))
-    (ensures (fun h0 w h1 ->
-      B.live h1 b /\
-      M.(modifies loc_none h0 h1) /\
-      w == Spec.ws a (B.as_seq h0 b) (U32.v t)))
-let rec ws a b t =
-  if U32.lt t 16ul then
-    b.(t)
-  else
-    let t16 = ws a b (U32.sub t 16ul) in
-    let t15 = ws a b (U32.sub t 15ul) in
-    let t7  = ws a b (U32.sub t 7ul) in
-    let t2  = ws a b (U32.sub t 2ul) in
+let ws a b ws =
+  let h0 = ST.get () in
+  let inv h1 (i: nat): Type0 =
+    let b = B.as_seq h0 b in
+    i <= Spec.size_k_w a /\
+    M.(modifies (loc_buffer ws) h0 h1) /\
+    S.equal (S.slice (B.as_seq h1 ws) 0 i) (S.init i (Spec.ws a b))
+  in
+  let f (i: U32.t { U32.(0 <= v i /\ v i < Spec.size_k_w a) }):
+    ST.Stack unit
+      (requires (fun h -> inv h (U32.v i)))
+      (ensures (fun h0 _ h1 -> U32.(inv h0 (v i) /\ inv h1 (v i + 1))))
+  =
+    if U32.(i <^ 16ul) then begin
+      (**) let h1 = ST.get () in
+      ws.(i) <- b.(i);
+      (**) let h2 = ST.get () in
+      (**) init_next (B.as_seq h2 ws) (Spec.ws a (B.as_seq h0 b)) (U32.v i)
+    end else
+      let h1 = ST.get () in
+      let t16 = ws.(U32.sub i 16ul) in
+      let t15 = ws.(U32.sub i 15ul) in
+      let t7  = ws.(U32.sub i 7ul) in
+      let t2  = ws.(U32.sub i 2ul) in
 
-    let s1 = Spec._sigma1 a t2 in
-    let s0 = Spec._sigma0 a t15 in
-    Spec.word_add_mod a s1 (Spec.word_add_mod a t7 (Spec.word_add_mod a s0 t16))
+      // JP: TODO, understand why this is not going through.
+      (**) assert (S.index (B.as_seq h1 ws) (U32.v i - 16) ==
+      (**)   S.index (S.init (U32.v i) (Spec.ws a (B.as_seq h0 b))) (U32.v i - 16));
+      (**) assert (t16 == Spec.ws a (B.as_seq h0 b) (U32.v i - 16));
+      (**) assert (S.index (B.as_seq h1 ws) (U32.v i - 15) ==
+      (**)   S.index (S.init (U32.v i) (Spec.ws a (B.as_seq h0 b))) (U32.v i - 15));
+      (**) assert (t15 == Spec.ws a (B.as_seq h0 b) (U32.v i - 15));
+      (**) assert (S.index (B.as_seq h1 ws) (U32.v i - 7) ==
+      (**)   S.index (S.init (U32.v i) (Spec.ws a (B.as_seq h0 b))) (U32.v i - 7));
+      (**) assert (t7 == Spec.ws a (B.as_seq h0 b) (U32.v i - 7));
+      (**) assert (S.index (B.as_seq h1 ws) (U32.v i - 2) ==
+      (**)   S.index (S.init (U32.v i) (Spec.ws a (B.as_seq h0 b))) (U32.v i - 2));
+      (**) assert (t2 == Spec.ws a (B.as_seq h0 b) (U32.v i - 2));
 
-#set-options "--max_fuel 0 --z3rlimit 50"
+      let s1 = Spec._sigma1 a t2 in
+      let s0 = Spec._sigma0 a t15 in
+      let w = Spec.word_add_mod a s1 (Spec.word_add_mod a t7 (Spec.word_add_mod a s0 t16)) in
+      ws.(i) <- w;
+      (**) let h2 = ST.get () in
+      (**) init_next (B.as_seq h2 ws) (Spec.ws a (B.as_seq h0 b)) (U32.v i)
+  in
+  C.Loops.for 0ul (U32.uint_to_t (Spec.size_k_w a)) inv f
+
+#set-options "--max_fuel 0"
 
 let hash_w (a: sha2_alg) =
   b:B.buffer (word a) { B.length b = size_hash_w a }
@@ -178,16 +247,20 @@ let add = Spec.word_add_mod
 val shuffle_core (a: sha2_alg)
   (block: block_w a)
   (hash: hash_w a)
+  (ws: ws_w a)
   (t: U32.t { U32.v t < Spec.size_k_w a }):
   ST.Stack unit
     (requires (fun h ->
-      B.live h block /\ B.live h hash /\
-      B.disjoint block hash))
+      let b = B.as_seq h block in
+      B.live h block /\ B.live h hash /\ B.live h ws /\
+      B.disjoint block hash /\ B.disjoint block ws /\ B.disjoint hash ws /\
+      B.as_seq h ws == S.init (Spec.size_k_w a) (Spec.ws a b)))
     (ensures (fun h0 _ h1 ->
       M.(modifies (loc_buffer hash) h0 h1) /\
       B.as_seq h1 hash == Spec.shuffle_core a (B.as_seq h0 block) (B.as_seq h0 hash) (U32.v t)))
 
-let shuffle_core a block hash t =
+#set-options "--z3rlimit 50"
+let shuffle_core a block hash ws t =
   let a0 = hash.(0ul) in
   let b0 = hash.(1ul) in
   let c0 = hash.(2ul) in
@@ -197,7 +270,9 @@ let shuffle_core a block hash t =
   let g0 = hash.(6ul) in
   let h0 = hash.(7ul) in
 
-  let t1 = add a h0 (add a (Spec._Sigma1 a e0) (add a (Spec._Ch a e0 f0 g0) (add a (k0 a).(t) (ws a block t)))) in
+  let w = ws.(t) in
+
+  let t1 = add a h0 (add a (Spec._Sigma1 a e0) (add a (Spec._Ch a e0 f0 g0) (add a (k0 a).(t) w))) in
   let t2 = add a (Spec._Sigma0 a a0) (Spec._Maj a a0 b0 c0) in
 
   hash.(0ul) <- add a t1 t2;
@@ -215,11 +290,13 @@ let shuffle_core a block hash t =
   (**) assert_norm (List.Tot.length l = 8);
   (**) S.intro_of_list #(word a) (B.as_seq h hash) l
 
-val shuffle: a:sha2_alg -> block:block_w a -> hash:hash_w a ->
+val shuffle: a:sha2_alg -> block:block_w a -> hash:hash_w a -> ws:ws_w a ->
   ST.Stack unit
     (requires (fun h ->
-      B.live h block /\ B.live h hash /\
-      B.disjoint block hash))
+      let b = B.as_seq h block in
+      B.live h block /\ B.live h hash /\ B.live h ws /\
+      B.disjoint block hash /\ B.disjoint block ws /\ B.disjoint hash ws /\
+      B.as_seq h ws == S.init (Spec.size_k_w a) (Spec.ws a b)))
     (ensures (fun h0 _ h1 ->
       M.(modifies (loc_buffer hash) h0 h1 /\
       B.as_seq h1 hash == Spec.shuffle a (B.as_seq h0 hash) (B.as_seq h0 block))))
@@ -227,14 +304,14 @@ val shuffle: a:sha2_alg -> block:block_w a -> hash:hash_w a ->
 inline_for_extraction
 let size_k_w (a: sha2_alg) = U32.uint_to_t (Spec.size_k_w a)
 
-let shuffle a block hash =
+let shuffle a block hash ws =
   let h0 = ST.get () in
   let inv (h1: HS.mem) (i: nat) =
     let block = B.as_seq h0 block in
     M.(modifies (loc_buffer hash) h0 h1) /\
     i <= Spec.size_k_w a /\
     B.as_seq h1 hash ==
-      Spec.Loops.repeat_range_spec 0 i (Spec.shuffle_core a block) (B.as_seq h0 hash)
+      Spec.Loops.repeat_range 0 i (Spec.shuffle_core a block) (B.as_seq h0 hash)
   in
   let f (i: U32.t { U32.(0 <= v i /\ v i < Spec.size_k_w a)}):
     ST.Stack unit
@@ -242,13 +319,13 @@ let shuffle a block hash =
       (ensures (fun h0 _ h1 ->
         U32.(inv h0 (v i) /\ inv h1 (v i + 1))))
   =
-    let h1 = ST.get () in
-    shuffle_core a block hash i;
-    let h2 = ST.get () in
-    let block0 = B.as_seq h0 block in
-    let hash0 = B.as_seq h0 hash in
-    Spec.Loops.lemma_repeat_range_spec 0 (U32.v i + 1) (Spec.shuffle_core a block0)
+    (**) let h1 = ST.get () in
+    shuffle_core a block hash ws i;
+    (**) let h2 = ST.get () in
+    (**) let block0 = B.as_seq h0 block in
+    (**) let hash0 = B.as_seq h0 hash in
+    (**) Spec.Loops.repeat_range_induction 0 (U32.v i + 1) (Spec.shuffle_core a block0)
       hash0
   in
-  Spec.Loops.lemma_repeat_range_0 0 0 (Spec.shuffle_core a (B.as_seq h0 block)) (B.as_seq h0 hash);
+  Spec.Loops.repeat_range_base 0 (Spec.shuffle_core a (B.as_seq h0 block)) (B.as_seq h0 hash);
   C.Loops.for 0ul (size_k_w a) inv f
